WIP

code/ecdsap256/Hacl.Impl.P256.Core.fst
@@ -570,128 +570,51 @@ let points_radix_16_list : x:list uint64{List.Tot.length x == 128} =
     u64 0x0; u64 0x0; u64 0x0; u64 0x0; 
     u64 0x0; u64 0x0; u64 0x0; u64 0x0; 
 
-u64 0x1fb38ab1388ad777; 
-u64 0x1dfee06615fa309d; 
-u64 0xfcac986c3afea4a7; 
-u64 0xdf65c2da29fb821a; 
-u64 0xeff44e23f63f8f6d; 
-u64 0xaa02cd3ed4b681a4; 
-u64 0xdd5fda3363818af8; 
-u64 0xfc53bc2629fbf0b3; 
-u64 0x12631d721b91beea; 
-u64 0x5f73f2d3a11a09f8; 
-u64 0xac41f54484d5fcd8; 
-u64 0x86578e5c56025df4; 
-u64 0x577c956b15ed6b5a; 
-u64 0xb59c5f77982d848; 
-u64 0xb7c5e2c190fcdcc2; 
-u64 0x7d64d13ef1c91ffd; 
-u64 0xd40c2d6273f9d9f1; 
-u64 0x4dc6f628063ef17c; 
-u64 0x498e81df7ab17aa5; 
-u64 0xabb2a5026f17173c; 
-u64 0x4a3d7527f6739ef3; 
-u64 0xd941003268184c91; 
-u64 0xd2d458b8d401508b; 
-u64 0xb7437ab810ac5451; 
-u64 0x5256d9bdab491252; 
-u64 0x972d326eb1084c12; 
-u64 0xc3e96455e2ec3bfa; 
-u64 0xb75c723b549a10ff; 
-u64 0x9d9185f9f8a18961; 
-u64 0x2200a07b8589ba82; 
-u64 0x637b9d96fd4e9f5e; 
-u64 0xce75bfb2575e6cfa; 
-u64 0x7dd4477db8b77c7d; 
-u64 0x80818a776e5503b0; 
-u64 0x6fc7d58fb59581d; 
-u64 0xd899fb87efe43022; 
-u64 0x23b9912111694135; 
-u64 0x7e5de7bac33fa1c8; 
-u64 0xb3b83722a70e7d43; 
-u64 0xf06cfecbfb9bb38f; 
-u64 0xaa39277dfa93656; 
-u64 0x3dabb6cce67c5201; 
-u64 0x473ffb8bf1f94677; 
-u64 0xb9f0b93637453e56; 
-u64 0x8fce12ec20958fb2; 
-u64 0xcc16d74ff7786061; 
-u64 0x3678438a8235d096; 
-u64 0xe39ea044f06b43f6; 
-u64 0xbb40bdb5775c9950; 
-u64 0xd244a74cdc703cdd; 
-u64 0x83dc1b8a6105dd53; 
-u64 0x38d9d50d49ef0437; 
-u64 0x58be44eba6096472; 
-u64 0x960afaec386fa5c5; 
-u64 0x1440032e000134b9; 
-u64 0x601e721454d6ba96; 
-u64 0x79ec42228671b9b6; 
-u64 0xfdc00dc48df9e25c; 
-u64 0x44500833d71d2e77; 
-u64 0x2bda4c3c0bc103d5; 
-u64 0x51528408aa925d53; 
-u64 0xefcb55b9c2f3a37d; 
-u64 0x9f28f6bb9846c915; 
-u64 0xe1547ce1d8340e55; 
-u64 0x97e310c1995b3ed2; 
-u64 0xed861937196256e6; 
-u64 0x1c6762abff2c65f2; 
-u64 0x268345e0978fcedd; 
-u64 0x35ca2e572b784881; 
-u64 0x28ac888da0acd1b7; 
-u64 0x305640dc06a41baf; 
-u64 0x997c6fd2cb671bfb; 
-u64 0xf40d9eaf4a31e15a; 
-u64 0x8991dd7d54cfe03a; 
-u64 0x4889a3463a8deb0c; 
-u64 0x4cbf48092cd0a1fa; 
-u64 0xc6965c4fbe18fb8c; 
-u64 0x1d499d0cb216fa84; 
-u64 0x8d5fe52c705dd3eb; 
-u64 0x812b268f84313b34; 
-u64 0x313b58808261591a; 
-u64 0xc2c322508f53d933; 
-u64 0xa49ef3f95094ed1b; 
-u64 0x13e326786e98c63; 
-u64 0x34be8167cd460429; 
-u64 0x698a328099a6b31; 
-u64 0xb9be3ba51b0c922d; 
-u64 0xe59cca03f7674ed; 
-u64 0x4fbf7e505d3aca7c; 
-u64 0x2f4f8ba62020715; 
-u64 0x840502262ac1ec42; 
-u64 0xb8e0532775197de7; 
-u64 0x9142a358cf4e9b4b; 
-u64 0xc86a3c567e5d8626; 
-u64 0xd4051282b4a7992a; 
-u64 0xe7573c5999e3974e; 
-u64 0xd814a606da7bd76b; 
-u64 0x15604730f38cb788; 
-u64 0xbd195f868fbdd6c4; 
-u64 0xdb96f5b00a51d3f7; 
-u64 0xe1385c8a9b507fea; 
-u64 0x878e27813ee7310; 
-u64 0x6d7d8b12aea7e096; 
-u64 0x54978ad11e2f5cca; 
-u64 0x49fffd6c3c4d07d4; 
-u64 0x703638f71fab7a5d; 
-u64 0xbed6e367fcc73960; 
-u64 0x215e161835a61d75; 
-u64 0xe52288a5e87a660b; 
-u64 0xf1d127ee3c802cb5; 
-u64 0xccde3c6aafc46044; 
-u64 0xdc11c08ef14cff32; 
-u64 0x29216f9ceca46668; 
-u64 0x22e584a3b2891c5e; 
-u64 0xe6deecd7810f6d87; 
-u64 0x6aff4b94a55659a3; 
-u64 0x12b59bb6d2e9f876; 
-u64 0x27ed01943aa02eab; 
-u64 0x8d6d420841f57075; 
-u64 0xe7b47285ef60a461;  
-  ] in
-  x
+    u64 0x1fb38ab1388ad777; u64 0x1dfee06615fa309d; u64 0xfcac986c3afea4a7; u64 0xdf65c2da29fb821a; 
+    u64 0xeff44e23f63f8f6d; u64 0xaa02cd3ed4b681a4; u64 0xdd5fda3363818af8; u64 0xfc53bc2629fbf0b3; 
+
+    u64 0x12631d721b91beea; u64 0x5f73f2d3a11a09f8; u64 0xac41f54484d5fcd8; u64 0x86578e5c56025df4; 
+    u64 0x577c956b15ed6b5a; u64 0xb59c5f77982d848; u64 0xb7c5e2c190fcdcc2; u64 0x7d64d13ef1c91ffd; 
+
+    u64 0xd40c2d6273f9d9f1; u64 0x4dc6f628063ef17c; u64 0x498e81df7ab17aa5; u64 0xabb2a5026f17173c; 
+    u64 0x4a3d7527f6739ef3; u64 0xd941003268184c91; u64 0xd2d458b8d401508b; u64 0xb7437ab810ac5451; 
+
+    u64 0x5256d9bdab491252; u64 0x972d326eb1084c12; u64 0xc3e96455e2ec3bfa; u64 0xb75c723b549a10ff; 
+    u64 0x9d9185f9f8a18961; u64 0x2200a07b8589ba82; u64 0x637b9d96fd4e9f5e; u64 0xce75bfb2575e6cfa; 
+
+    u64 0x7dd4477db8b77c7d; u64 0x80818a776e5503b0; u64 0x6fc7d58fb59581d; u64 0xd899fb87efe43022; 
+    u64 0x23b9912111694135; u64 0x7e5de7bac33fa1c8; u64 0xb3b83722a70e7d43; u64 0xf06cfecbfb9bb38f; 
+
+    u64 0xaa39277dfa93656; u64 0x3dabb6cce67c5201; u64 0x473ffb8bf1f94677; u64 0xb9f0b93637453e56; 
+    u64 0x8fce12ec20958fb2; u64 0xcc16d74ff7786061; u64 0x3678438a8235d096; u64 0xe39ea044f06b43f6; 
+
+    u64 0xbb40bdb5775c9950; u64 0xd244a74cdc703cdd; u64 0x83dc1b8a6105dd53; u64 0x38d9d50d49ef0437; 
+    u64 0x58be44eba6096472; u64 0x960afaec386fa5c5; u64 0x1440032e000134b9; u64 0x601e721454d6ba96; 
+
+    u64 0x79ec42228671b9b6; u64 0xfdc00dc48df9e25c; u64 0x44500833d71d2e77; u64 0x2bda4c3c0bc103d5; 
+    u64 0x51528408aa925d53; u64 0xefcb55b9c2f3a37d; u64 0x9f28f6bb9846c915; u64 0xe1547ce1d8340e55; 
+
+    u64 0x97e310c1995b3ed2; u64 0xed861937196256e6; u64 0x1c6762abff2c65f2; u64 0x268345e0978fcedd; 
+    u64 0x35ca2e572b784881; u64 0x28ac888da0acd1b7; u64 0x305640dc06a41baf; u64 0x997c6fd2cb671bfb; 
+
+    u64 0xf40d9eaf4a31e15a; u64 0x8991dd7d54cfe03a; u64 0x4889a3463a8deb0c; u64 0x4cbf48092cd0a1fa; 
+    u64 0xc6965c4fbe18fb8c; u64 0x1d499d0cb216fa84; u64 0x8d5fe52c705dd3eb; u64 0x812b268f84313b34; 
+
+    u64 0x313b58808261591a; u64 0xc2c322508f53d933; u64 0xa49ef3f95094ed1b; u64 0x13e326786e98c63; 
+    u64 0x34be8167cd460429; u64 0x698a328099a6b31; u64 0xb9be3ba51b0c922d; u64 0xe59cca03f7674ed; 
+    
+    u64 0x4fbf7e505d3aca7c; u64 0x2f4f8ba62020715; u64 0x840502262ac1ec42; u64 0xb8e0532775197de7; 
+    u64 0x9142a358cf4e9b4b; u64 0xc86a3c567e5d8626; u64 0xd4051282b4a7992a; u64 0xe7573c5999e3974e;
+    
+    u64 0xd814a606da7bd76b; u64 0x15604730f38cb788; u64 0xbd195f868fbdd6c4; u64 0xdb96f5b00a51d3f7; 
+    u64 0xe1385c8a9b507fea; u64 0x878e27813ee7310; u64 0x6d7d8b12aea7e096; u64 0x54978ad11e2f5cca; 
+    
+    u64 0x49fffd6c3c4d07d4; u64 0x703638f71fab7a5d; u64 0xbed6e367fcc73960; u64 0x215e161835a61d75; 
+    u64 0xe52288a5e87a660b; u64 0xf1d127ee3c802cb5; u64 0xccde3c6aafc46044; u64 0xdc11c08ef14cff32; 
+
+    u64 0x29216f9ceca46668; u64 0x22e584a3b2891c5e; u64 0xe6deecd7810f6d87; u64 0x6aff4b94a55659a3; 
+   u64 0x12b59bb6d2e9f876; u64 0x27ed01943aa02eab; u64 0x8d6d420841f57075; u64 0xe7b47285ef60a461;  
+  ] in x
 
 
 
@@ -724,7 +647,7 @@ let getScalar #a scalar i =
   
 
 
-let montgomery_ladder_step_radix p tempBuffer scalar i =  
+let montgomery_ladder_step_radix_precomputed p tempBuffer scalar i =  
   let bits: uint32 = getScalar scalar (i) in 
 
   let pointToAdd = sub points_radix_16 (bits *. size 8) (size 8) in 
@@ -738,17 +661,29 @@ let montgomery_ladder_step_radix p tempBuffer scalar i =
   Hacl.Impl.P256.MixedPointAdd.point_add_mixed p pointToAdd p tempBuffer
 
 
+let montgomery_ladder_step_radix p tempBuffer precomputedTable scalar i =  
+  let bits = getScalar scalar i in 
+
+  let pointToAdd = sub precomputedTable (bits *. size 12) (size 12) in 
+  
+  point_double p p tempBuffer;
+  point_double p p tempBuffer;
+  point_double p p tempBuffer;
+  point_double p p tempBuffer;
+
+  point_add pointToAdd p p tempBuffer
+
 
 
 inline_for_extraction noextract
-val montgomery_ladder_2: #buf_type: buftype -> p: point -> 
+val montgomery_ladder_2_precomputed: #buf_type: buftype -> p: point -> 
   scalar: lbuffer_t buf_type uint8 (size 32) -> 
   tempBuffer:  lbuffer uint64 (size 88)  -> 
   Stack unit
   (requires fun h -> True )
   (ensures fun h0 _ h1 -> modifies (loc p |+| loc tempBuffer) h0 h1)
 
-let montgomery_ladder_2 #a p scalar tempBuffer =  
+let montgomery_ladder_2_precomputed #a p scalar tempBuffer =  
  let h0 = ST.get() in 
 
   [@inline_let]
@@ -762,8 +697,91 @@ let montgomery_ladder_2 #a p scalar tempBuffer =
 
   for 0ul 64ul inv 
     (fun i -> let h2 = ST.get() in
-      montgomery_ladder_step_radix p tempBuffer scalar i
+      montgomery_ladder_step_radix_precomputed p tempBuffer scalar i
     )
+
+
+val uploadZeroPoint: p: point -> Stack unit 
+  (requires fun h -> True)
+  (ensures fun h0 _ h1 -> True)
+
+let uploadZeroPoint p = 
+  uploadZeroImpl (sub p (size 0) (size 4));
+  uploadZeroImpl (sub p (size 4) (size 4));
+  uploadZeroImpl (sub p (size 8) (size 4))
+
+
+val generatePrecomputedTable: b: lbuffer uint64 (size 192) -> publicKey: point ->
+  tempBuffer: lbuffer uint64 (size 88) -> Stack unit  
+  (requires fun h -> True)
+  (ensures fun h0 _ h1 -> True)
+
+let generatePrecomputedTable b publicKey tempBuffer = 
+  let point0 = sub b (size 0) (size 12) in 
+  let point1 = sub b (size 12) (size 12) in 
+  let point2 = sub b (size 24) (size 12) in 
+  let point3 = sub b (size 36) (size 12) in 
+  let point4 = sub b (size 48) (size 12) in 
+  let point5 = sub b (size 60) (size 12) in 
+  let point6 = sub b (size 72) (size 12) in 
+  let point7 = sub b (size 84) (size 12) in 
+  let point8 = sub b (size 96) (size 12) in 
+  let point9 = sub b (size 108) (size 12) in 
+  let point10 = sub b (size 120) (size 12) in 
+  let point11 = sub b (size 132) (size 12) in 
+  let point12 = sub b (size 144) (size 12) in 
+  let point13 = sub b (size 156) (size 12) in 
+  let point14 = sub b (size 168) (size 12) in 
+  let point15 = sub b (size 180) (size 12) in 
+
+  uploadZeroPoint point0;
+  copy_point publicKey point1;
+  point_double publicKey point2 tempBuffer;
+  point_add point2 point1 point3 tempBuffer;
+  point_double point2 point4 tempBuffer;
+  point_add point4 point1 point5 tempBuffer;
+  point_double point3 point6 tempBuffer;
+  point_add point6 point1 point7 tempBuffer;
+  point_double point4 point8 tempBuffer;
+  point_add point8 point1 point9 tempBuffer;
+  point_double point5 point10 tempBuffer;
+  point_add point10 point1 point11 tempBuffer;
+  point_double point6 point12 tempBuffer;
+  point_add point12 point1 point13 tempBuffer;
+  point_double point7 point14 tempBuffer;
+  point_add point14 point1 point15 tempBuffer
+
+
+
+inline_for_extraction noextract
+val montgomery_ladder_2: #buf_type: buftype -> p: point -> 
+  scalar: lbuffer_t buf_type uint8 (size 32) -> 
+  tempBuffer:  lbuffer uint64 (size 88)  -> 
+  Stack unit
+  (requires fun h -> True )
+  (ensures fun h0 _ h1 -> modifies (loc p |+| loc tempBuffer) h0 h1)
+
+let montgomery_ladder_2 #a p scalar tempBuffer =  
+ let h0 = ST.get() in 
+   push_frame();
+     let bufferPrecomputed = create (size 192) (u64 0) in 
+     generatePrecomputedTable bufferPrecomputed p tempBuffer;
+
+     [@inline_let]
+     let spec_ml h0 = _ml_step (as_seq h0 scalar) in 
+
+     [@inline_let] 
+     let acc (h:mem) : GTot (point_nat_prime) = (fromDomainPoint(point_prime_to_coordinates (as_seq h p)))  in 
+
+     [@inline_let]
+     let inv h (i: nat {i <= 64}) = True in 
+
+     for 0ul 64ul inv 
+       (fun i -> let h2 = ST.get() in
+	 montgomery_ladder_step_radix p tempBuffer bufferPrecomputed scalar i
+       );
+   pop_frame()
+
 
 
 
@@ -863,8 +881,7 @@ val scalarMultiplication_t: #t:buftype -> p: point -> result: point ->
 
 
 let scalarMultiplication_t #t p result scalar tempBuffer  = 
-(* 
-
+(*
     let h0 = ST.get() in 
   let q = sub tempBuffer (size 0) (size 12) in 
   zero_buffer q;
@@ -888,8 +905,9 @@ let scalarMultiplication_t #t p result scalar tempBuffer  =
     let h3 = ST.get() in 
     lemma_point_to_domain h0 h2 p result;
     lemma_pif_to_domain h2 q;
-  norm q result buff; 
+  norm result result buff; 
     lemma_coord h3 q
+
 
 
 
@@ -968,20 +986,6 @@ let scalarMultiplicationWithoutNorm p result scalar tempBuffer =
     lemma_pif_to_domain h2 q
     
 
-let secretToPublic result scalar tempBuffer = 
-  push_frame(); 
-       let basePoint = create (size 12) (u64 0) in 
-    uploadBasePoint basePoint;
-      let q = sub tempBuffer (size 0) (size 12) in 
-      let buff = sub tempBuffer (size 12) (size 88) in 
-    zero_buffer q; 
-      let h1 = ST.get() in 
-      lemma_pif_to_domain h1 q;
-    montgomery_ladder q basePoint scalar buff; 
-    norm q result buff;  
-  pop_frame()
-
-
 let secretToPublicWithoutNorm result scalar tempBuffer = 
     push_frame(); 
       let basePoint = create (size 12) (u64 0) in 
@@ -1023,7 +1027,7 @@ let secretToPublic m result scalar tempBuffer =
       uploadBasePoint basePoint;
     montgomery_ladder result basePoint scalar buff
   |Radix4 ->
-      montgomery_ladder_2 result scalar buff
+      montgomery_ladder_2_precomputed result scalar buff
    end; 
   (* zero_buffer result; *)
     let h1 = ST.get() in 
@@ -1032,20 +1036,6 @@ let secretToPublic m result scalar tempBuffer =
   norm result result buff
 
 
-(*
-let secretToPublic m result scalar tempBuffer = 
-  push_frame(); 
-       let basePoint = create (size 12) (u64 0) in 
-    (* uploadBasePoint basePoint; *)
-      let q = sub tempBuffer (size 0) (size 12) in 
-      let buff = sub tempBuffer (size 12) (size 88) in 
-    zero_buffer q; 
-      let h1 = ST.get() in 
-      lemma_pif_to_domain h1 q;
-    montgomery_ladder_2 result scalar buff; 
-    norm result result buff;  
-  pop_frame()
-*)
 
 let secretToPublicWithoutNorm result scalar tempBuffer = 
     push_frame(); 
