code/ecdsap256/Hacl.Impl.P256.DH.fsti
@@ -32,7 +32,8 @@ val ecp256dh_i:
 
 inline_for_extraction noextract
 val ecp256dh_r:
-    result:lbuffer uint8 (size 64)
+  m: montgomery_ladder_mode
+  -> result:lbuffer uint8 (size 64)
   -> pubKey:lbuffer uint8 (size 64)
   -> scalar:lbuffer uint8 (size 32)
   -> Stack bool
